AccessProp.v
@@ -20,7 +20,7 @@ Proof.
   intros * Hnacc Hacc. induction Hacc;
   inversion_not_access Hnacc; eauto using access.
   decompose sum (lt_eq_lt_dec ad' (length m)); subst;
-  do 3 (rewrite_array TM_Unit); eauto using access; try contradiction.
+  do 3 simpl_array; eauto using access; try contradiction.
   auto_specialize. inversion_access.
 Qed.
 
@@ -31,7 +31,8 @@ Proof.
   intros * Hnacc F. remember (length m) as ad.
   induction F; inversion Heqad; subst; inversion_not_access Hnacc.
   decompose sum (lt_eq_lt_dec ad' (length m)); subst; try lia;
-  do 2 (rewrite_array TM_Unit); eauto. inversion_access.
+  do 2 simpl_array; eauto.
+  simpl_array. eauto.
 Qed.
 
 Lemma mem_add_nacc_lt : forall m t ad v,
@@ -41,7 +42,7 @@ Lemma mem_add_nacc_lt : forall m t ad v,
 Proof.
   intros * Hnacc1 Hnacc2 F. induction F; inversion_not_access Hnacc2.
   decompose sum (lt_eq_lt_dec ad' (length m)); subst;
-  do 2 rewrite_term_array;
+  do 2 simpl_array;
   inversion_not_access Hnacc1.
   eapply IHF; eapply not_access_iff; eauto using not_access.
 Qed.
@@ -55,7 +56,7 @@ Proof.
   induction Hacc; inversion Heqm'; subst; inversion_not_access Hnacc.
   eapply access_mem; trivial.
   decompose sum (lt_eq_lt_dec ad' (length m)); subst;
-  do 2 (rewrite_array TM_Unit); eauto;
+  do 2 simpl_array; eauto;
   rewrite (get_default TM_Unit) in *; eauto using access; lia.
 Qed.
 
@@ -66,16 +67,10 @@ Proof.
   intros * Hacc. induction Hacc; eauto using access.
   destruct (Nat.eq_dec ad ad'); subst; eauto using access.
   eapply access_mem; trivial.
-  decompose sum (lt_eq_lt_dec ad' (length m)); subst.
-  - rewrite_array TM_Unit; trivial.
-  - rewrite (get_default TM_Unit) in IHHacc; try lia. inversion_access.
-  - rewrite (get_default TM_Unit) in IHHacc; try lia. inversion_access.
+  decompose sum (lt_eq_lt_dec ad' (length m)); subst;
+  simpl_array; trivial;
+  do 2 simpl_array; inversion_access.
 Qed.
-
-Module Mem.
-  Module Set_.
-  End Set_.
-End Mem.
 
 (* ------------------------------------------------------------------------- *)
 (* Step                                                                      *)
@@ -239,7 +234,7 @@ Proof.
   intros. induction_step; inversion_access;
   eauto using access, mem_add_preserves_access.
   destruct (Nat.eq_dec ad (length m)); subst; eauto using access.
-  eapply access_mem; trivial. rewrite_term_array.
+  eapply access_mem; trivial. simpl_array.
   eauto using mem_add_preserves_access.
 Qed.
 
@@ -253,7 +248,7 @@ Proof.
   intros * Hva ? Hnacc ?.
   induction_step; inversion_va; inversion_not_access Hnacc;
   intros F; inversion_access;
-  try solve [unfold not in *; eauto]; try rewrite_term_array;
+  try solve [unfold not in *; eauto]; try simpl_array;
   match goal with F : access (_ +++ _) _ _ |- _ => contradict F end;
   eauto using mem_add_nacc_lt, va_nacc_length.
 Qed.
@@ -267,7 +262,7 @@ Lemma step_alloc_inherits_acc : forall m t t' ad v,
 Proof.
   intros. induction_step;
   inversion_va; inversion_access; eauto using access;
-  try lia; try rewrite_term_array;
+  try lia; try simpl_array;
   eauto using mem_add_inherits_access, va_nacc_length, access.
 Qed.
 
@@ -280,7 +275,7 @@ Lemma step_alloc_creates_acc : forall ad v m t t',
 Proof.
   intros * ? Hnacc ? ?.
   induction_step; inversion_va; inversion_not_access Hnacc; inversion_access;
-  eauto; try rewrite_term_array;
+  eauto; try simpl_array;
   match goal with F : access (_ +++ _) _ _ |- _ => contradict F end;
   eauto using mem_add_nacc_lt, va_nacc_length.
 Qed.
@@ -346,7 +341,7 @@ Lemma mem_set_preserves_acc2 : forall m t ad ad' v,
 Proof.
   intros * Hnacc Hacc.  remember (m[ad' <- v]) as m'.
   induction Hacc; inversion_subst_clear Heqm'; inversion_not_access Hnacc;
-  try (do 2 rewrite_term_array);
+  try (do 2 simpl_array);
   eauto using access.
 Qed.
 
@@ -379,7 +374,7 @@ Proof.
     destruct (Nat.eq_dec ad' ad) as [? | Hneq]; subst;
     try (assert (ad < length m) by eauto)
   end;
-  do 2 rewrite_term_array; eauto using access.
+  do 2 simpl_array; eauto using access.
 Qed.
 
 Local Lemma step_write_value_acc : forall m t t' ad ad' v,
